src/lib/state/DY.Lib.State.Tagged.fst
@@ -146,6 +146,14 @@ let tagged_state_was_set tr tag prin sess_id content =
   let full_content_bytes = serialize tagged_state full_content in
   state_was_set tr prin sess_id full_content_bytes
 
+[@@ "opaque_to_smt"]
+val tagged_state_was_set_at: trace -> timestamp -> string -> principal -> state_id -> bytes -> prop
+let tagged_state_was_set_at tr ts tag prin sess_id content =
+  let full_content = {tag; content;} in
+  let full_content_bytes = serialize tagged_state full_content in
+  state_was_set_at tr ts prin sess_id full_content_bytes
+
+
 (*** API for tagged sessions ***)
 
 [@@ "opaque_to_smt"]
@@ -223,24 +231,47 @@ let get_tagged_state_invariant invs tag spred prin sess_id tr =
 
 (*** Theorem ***)
 
+// val tagged_state_was_set_implies_pred:
+//   invs:protocol_invariants -> tr:trace ->
+//   tag:string -> spred:local_bytes_state_predicate ->
+//   prin:principal -> sess_id:state_id -> content:bytes ->
+//   Lemma
+//   (requires
+//     tagged_state_was_set tr tag prin sess_id content /\
+//     trace_invariant tr /\
+//     has_local_bytes_state_predicate invs (tag, spred)
+//   )
+//   (ensures spred.pred tr prin sess_id content)
+//   [SMTPat (tagged_state_was_set tr tag prin sess_id content);
+//    SMTPat (trace_invariant tr);
+//    SMTPat (has_local_bytes_state_predicate invs (tag, spred));
+//   ]
+// let tagged_state_was_set_implies_pred invs tr tag spred prin sess_id content =
+//   reveal_opaque (`%tagged_state_was_set) (tagged_state_was_set);
+//   let full_content = {tag; content;} in
+//   parse_serialize_inv_lemma #bytes tagged_state full_content;
+//   let full_content_bytes: bytes = serialize tagged_state full_content in
+//   local_eq_global_lemma split_local_bytes_state_predicate_func state_pred tag spred (tr, prin, sess_id, full_content_bytes) (tr, prin, sess_id, content)
+
+
 val tagged_state_was_set_implies_pred:
-  invs:protocol_invariants -> tr:trace ->
+  invs:protocol_invariants -> tr:trace -> ts:timestamp{ts <= DY.Core.Trace.Type.length tr} ->
   tag:string -> spred:local_bytes_state_predicate ->
   prin:principal -> sess_id:state_id -> content:bytes ->
   Lemma
   (requires
-    tagged_state_was_set tr tag prin sess_id content /\
+    tagged_state_was_set_at tr ts tag prin sess_id content /\
     trace_invariant tr /\
     has_local_bytes_state_predicate invs (tag, spred)
   )
-  (ensures spred.pred tr prin sess_id content)
-  [SMTPat (tagged_state_was_set tr tag prin sess_id content);
+  (ensures spred.pred (prefix tr ts) prin sess_id content)
+  [SMTPat (tagged_state_was_set_at tr ts tag prin sess_id content);
    SMTPat (trace_invariant tr);
    SMTPat (has_local_bytes_state_predicate invs (tag, spred));
   ]
-let tagged_state_was_set_implies_pred invs tr tag spred prin sess_id content =
-  reveal_opaque (`%tagged_state_was_set) (tagged_state_was_set);
+let tagged_state_was_set_implies_pred invs tr ts tag spred prin sess_id content =
+  reveal_opaque (`%tagged_state_was_set_at) (tagged_state_was_set_at);
   let full_content = {tag; content;} in
   parse_serialize_inv_lemma #bytes tagged_state full_content;
   let full_content_bytes: bytes = serialize tagged_state full_content in
-  local_eq_global_lemma split_local_bytes_state_predicate_func state_pred tag spred (tr, prin, sess_id, full_content_bytes) (tr, prin, sess_id, content)
+  local_eq_global_lemma split_local_bytes_state_predicate_func state_pred tag spred (prefix tr ts, prin, sess_id, full_content_bytes) (prefix tr ts, prin, sess_id, content)
